feat: generalize pf(E) results to (subsets of) pf(B)

CombinatorialGames/Misere/Blocking.lean
@@ -263,6 +263,19 @@ instance : HasInt (ShortBlocking (G := G)) where
     { short := IsShort.intCast k
     , blocking := isBlocking_intCast k }
 
+
+class Blocking (A : G → Prop) where
+  isBlocking {g : G} (hA : A g) : IsBlocking g
+
+instance : Blocking (IsBlocking (G := G)) where
+  isBlocking := id
+
+instance : Blocking (ShortBlocking (G := G)) where
+  isBlocking h := h.blocking
+
+instance instBlockingOfDeadEnding (A : G → Prop) [DeadEnding A] : Blocking A where
+  isBlocking hA := isBlocking_of_isDeadEnding (DeadEnding.isDeadEnding hA)
+
 end Form
 
 namespace GameForm
@@ -387,5 +400,68 @@ This is [Davies, Miller, Milley (Lemma 4.5 on p. 26)][davies:SumsPFreeForms:2025
 -/
 instance : IntegerInvertible ShortBlocking where
   int_add_neg_misereEQ := int_add_neg_misereEQ_blocking
+
+mutual
+
+private theorem isBlockedEnd_left_strongTest_winsGoingFirst {x g : GameForm}
+    (hx : IsBlockedEnd .left x) (ht : IsStrongTest .left g) :
+    WinsGoingFirst .left (g + x) := by
+  have hxe : IsEnd .left x := isEnd_of_isBlockedEnd hx
+  rw [isStrongTest_def] at ht
+  rcases ht with hge | ⟨gl, hgl, hout, htgl, hgr⟩
+  · exact winsGoingFirst_of_isEnd (IsEnd.add_iff.mpr ⟨hge, hxe⟩)
+  · apply winsGoingFirst_of_moves
+    refine ⟨gl + x, add_right_mem_moves_add hgl x, ?_⟩
+    rw [Player.neg_left]
+    apply isBlockedEnd_left_strongTest_not_winsGoingFirst hx hout htgl
+    intro gr hgr'
+    exact hgr gr (by rw [Player.neg_left]; exact hgr')
+termination_by (x, g)
+decreasing_by form_wf
+
+private theorem isBlockedEnd_left_strongTest_not_winsGoingFirst {x g : GameForm}
+    (hx : IsBlockedEnd .left x) (hout : MisereOutcome g = .L)
+    (ht : IsStrongTest .left g)
+    (hr : ∀ gr ∈ moves .right g, IsStrongTest .left gr) :
+    ¬ WinsGoingFirst .right (g + x) := by
+  rw [not_winsGoingFirst_iff]
+  refine ⟨?_, ?_⟩
+  · rw [GameForm.isEndLike_iff_isEnd, IsEnd.add_iff]
+    rintro ⟨hgend, _⟩
+    exact (misereOutcome_L_iff_winsGoingFirst.mp hout).right
+      (winsGoingFirst_of_isEnd hgend)
+  · intro y hy
+    rw [Player.neg_right]
+    rw [moves_add] at hy
+    rcases hy with ⟨gr, hgr, rfl⟩ | ⟨xr, hxr, rfl⟩
+    · exact isBlockedEnd_left_strongTest_winsGoingFirst hx (hr gr hgr)
+    · rcases IsBlockedEnd.hereditary_def hx xr hxr with hxrbe | ⟨xrl, hxrl, hxrlbe⟩
+      · exact isBlockedEnd_left_strongTest_winsGoingFirst hxrbe ht
+      · apply winsGoingFirst_of_moves
+        exact ⟨g + xrl, add_left_mem_moves_add hxrl g,
+          isBlockedEnd_left_strongTest_not_winsGoingFirst hxrlbe hout ht hr⟩
+termination_by (x, g)
+decreasing_by form_wf
+
+end
+
+private theorem IsBlocking.left_strong_of_isStrongTest {g : GameForm}
+    (h_test : IsStrongTest .left g) :
+    Strong IsBlocking g .left := by
+  intro x hx h_isEnd
+  rw [GameForm.isEndLike_iff_isEnd] at h_isEnd
+  exact isBlockedEnd_left_strongTest_winsGoingFirst (isBlockedEnd_of_isBlocking hx h_isEnd) h_test
+
+/--
+This is one direction of [Davies, Milley (Theorem 3.1 on p. 7)][davies:OrderInversesMonoid:2026]
+-/
+theorem IsBlocking.strong_of_isStrongTest {p : Player} {g : GameForm}
+    (h_test : IsStrongTest p g) :
+    Strong IsBlocking g p := by
+  cases p
+  · exact left_strong_of_isStrongTest h_test
+  · rw [<-neg_neg g, IsStrongTest.neg_iff, Player.neg_right] at h_test
+    rw [<-neg_neg g, Strong.neg_iff, Player.neg_right]
+    exact left_strong_of_isStrongTest h_test
 
 end GameForm
