CombinatorialGames/Misere/PFreeDeadEnding.lean
@@ -11,10 +11,8 @@ public import CombinatorialGames.Misere.DeadEnding
 # $\mathscr{P}$-free dead-ending games
 
 The main results are
-* `reduction_ab_int`
 * `misereGE_of_int_le`
-* `misereGE_iff_promain_not_isEnd_left_int`
-* `misereGE_iff_promain_not_isEnd_left_right`
+* `isEnd_exists_intCast_misereEQ`
 -/
 
 public section
@@ -132,11 +130,8 @@ instance : OutcomeStable (IsDeadEnding (G := GameForm)) where
 
 abbrev PFreeDeadEnding (g : GameForm) : Prop := (PFreeSubset DeadEnding.ShortDeadEnding) g
 
-def PFreeDeadEnding.isDeadEnding {g : GameForm} (h_g : PFreeDeadEnding g) : IsDeadEnding g :=
-  h_g.mem.dead_ending
-
 instance : DeadEnding PFreeDeadEnding where
-  isDeadEnding h := h.isDeadEnding
+  isDeadEnding h := h.mem.dead_ending
 
 instance : Short PFreeDeadEnding where
   isShort h := h.mem.short
@@ -177,37 +172,21 @@ theorem misereGE_of_int_le (a b : ℤ) (h1 : a ≥ b) : b ≥m PFreeDeadEnding a
 theorem misereGE_of_nat_le (a b : ℕ) (h1 : a ≥ b) : b ≥m PFreeDeadEnding a :=
   OutcomeStable.misereGE_of_nat_le _ b a h1
 
-theorem a_one_MisereOutcome {a : ℤ} (h0 : 0 ≤ a) : MisereOutcome (!{{(a : GameForm)} | {1}}) = .R := by
-  rw [misereOutcome_R_iff_winsGoingFirst]
-  apply And.intro
-  · refine winsGoingFirst_of_moves ⟨1, ?_⟩
-    simp only [moves_ofSets, Set.mem_singleton_iff, Player.le_left, Player.neg_right, Player.le_left_eq, true_and]
-    rw [not_winsGoingFirst_iff]
-    apply And.intro (by simp)
-    simp
-  · rw [not_winsGoingFirst_iff]
-    simp [isEnd_def, h0]
+-- TODO: Move and maybe even @[simp]
+theorem misereOutcome_ne_P_iff_winsGoingFirst {g : GameForm} :
+    (MisereOutcome g ≠ .P) ↔ (WinsGoingFirst .right g ∨ WinsGoingFirst .left g) := by
+  have := (misereOutcome_P_iff_winsGoingFirst (g := g)).not
+  tauto
 
-theorem a_one_pfreeDeadEnding {a : ℤ} (h0 : 0 ≤ a) : PFreeDeadEnding (!{{(a : GameForm)} | {1}}) := by
-  apply PFreeSubset.mk
-  · exact
-    { dead_ending := by
-        unfold IsDeadEnding
-        apply And.intro <;> intro p <;> cases p
-        · simp [isEnd_def]
-        · simp [isEnd_def]
-        · simp
-        · simp
-      short := by
-        rw [isShort_def]
-        intro p; cases p
-        · simp
-        · simp
-    }
-  · unfold IsPFree
-    apply And.intro
-    · simp [a_one_MisereOutcome, h0]
-    · intro p; cases p <;> simp
+-- TODO: Move
+@[simp]
+theorem Set.insert_ne_empty {A : Type*} (x : A) (xs : Set A) : insert x xs ≠ ∅ := by
+  simp [<-Set.nonempty_iff_ne_empty']
+
+-- TODO: Move
+theorem not_isEnd_nonempty {p : Player} {g : GameForm} (h1 : ¬ IsEnd p g) : Nonempty (moves p g) := by
+  rw [isEnd_def] at h1
+  exact Set.nonempty_iff_ne_empty'.mpr h1
 
 theorem misereGE_of_maintenance_proviso
     {g h : GameForm} (hg : IsPFree g) (hh : IsPFree h)
@@ -217,63 +196,19 @@ theorem misereGE_of_maintenance_proviso
   refine Hereditary.misereGE_of_maintenance_proviso PFreeDeadEnding h_m_r h_m_l ?_ ?_
   · intro h_isEnd
     rw [GameForm.isEndLike_iff_isEnd] at h_isEnd
-    rw [PFree.strong_right_iff_misereOutcome_L hh]
+    rw [PFree.strong_iff_misereOutcome hh]
     exact h_p_r h_isEnd
   · intro h_isEnd
     rw [GameForm.isEndLike_iff_isEnd] at h_isEnd
-    rw [PFree.strong_left_iff_misereOutcome_R hg]
+    rw [PFree.strong_iff_misereOutcome hg]
     exact h_p_l h_isEnd
 
-theorem reduction_a_one_int {a : ℤ} (h0 : 0 ≤ a)
-    : (!{{(a : GameForm)} | {1}}) =m PFreeDeadEnding ((a + 1) : ℤ) := by
-  have h0' : 0 ≤ a + 1 := Int.le_add_one h0
-  have h0'' : 0 < a + 1 := Int.le_iff_lt_add_one.mp h0
-  refine MisereEq.of_antisymm ?_ ?_
-  · apply misereGE_of_maintenance_proviso (a_one_pfreeDeadEnding h0).isPFree (HasInt.has_int _)
-    · simpa [Maintenance, h0'] using misereGE_of_int_le (a + 1) 0 h0'
-    · simp only [Maintenance, moves_ofSets, Set.mem_singleton_iff, exists_eq_left]
-      intro hl h_hl
-      apply Or.inl
-      have h_hl := eq_sub_one_of_mem_leftMoves_intCast h_hl
-      rw [Int.add_sub_cancel a 1] at h_hl
-      simp [h_hl]
-    · simp [isEnd_def]
-    · simp [isEnd_def, h0]
-  · apply misereGE_of_maintenance_proviso (HasInt.has_int _) (a_one_pfreeDeadEnding h0).isPFree
-    · simp [Maintenance, h0']
-    · simp [Maintenance, h0'']
-    · intro h1 h2
-      rw [misereOutcome_L_iff_winsGoingFirst] at h2
-      absurd h2.right
-      apply winsGoingFirst_of_moves
-      simp
-    · simp [isEnd_def]
-
-private theorem reduction_ab_int.auxL {a b : ℤ} (h0 : 0 ≤ a) (h2 : 1 ≤ b) (h3 : b ≤ a + 2)
-    : (!{{(a : GameForm)} | {(b : GameForm)}}) ≥m PFreeDeadEnding (!{{(a : GameForm)} | {(1 : GameForm)}}) := by
-  apply Hereditary.misereGE_of_maintenance_proviso PFreeDeadEnding
-  · simp only [Maintenance, moves_ofSets, Set.mem_singleton_iff, exists_eq_left, forall_eq]
-    refine Or.inr ⟨((b - 1) : ℤ), leftMoves_intCast_zero_lt h2, ?_⟩
-    exact misereGE_rw_right (reduction_a_one_int h0) (misereGE_of_int_le (a + 1) (b - 1) (by omega))
-  · simp [Maintenance]
-  · simp [Proviso, isEnd_def]
-  · simp [Proviso, isEnd_def]
-
-private theorem reduction_ab_int.auxR (a : ℤ) {b : ℤ} (h0 : 1 ≤ b)
-    : (!{{(a : GameForm)} | {(1 : GameForm)}}) ≥m PFreeDeadEnding (!{{(a : GameForm)} | {(b : GameForm)}}) := by
-  apply Hereditary.misereGE_of_maintenance_proviso PFreeDeadEnding
-  · simp only [Maintenance, moves_ofSets, Set.mem_singleton_iff, exists_eq_left, forall_eq]
-    apply Or.inl
-    rw [<-Form.intCast_one]
-    exact misereGE_of_int_le b (1 : ℕ) h0
-  · simp [Maintenance]
-  · simp [Proviso, isEnd_def]
-  · simp [Proviso, isEnd_def]
-
-theorem reduction_ab_int (a b : ℤ) (h0 : 0 ≤ a) (h1 : 1 ≤ b) (h2 : b ≤ a + 2)
-    : (!{{(a : GameForm)} | {(b : GameForm)}}) =m PFreeDeadEnding ((a + 1) : ℤ) := by
-  refine MisereEQ.trans ?_ (reduction_a_one_int h0)
-  apply MisereEq.of_antisymm (reduction_ab_int.auxL h0 h1 h2) (reduction_ab_int.auxR a h1)
+-- TODO: Move
+@[simp]
+theorem isEnd_ofSets {p : Player}
+    {st : Player → Set GameForm} [Small (st .left)] [Small (st .right)] :
+  IsEnd p !{st} ↔ (st p = ∅) := by
+  simp [isEnd_def]
 
 lemma strong_left_of_misereOutcome_L {A : GameForm → Prop} [PFree A] [OutcomeStable A] {g : GameForm}
     (h1 : (PFreeSubset A) g) (h2 : MisereOutcome g = .L) : Strong (PFreeSubset A) g .left := by
@@ -294,117 +229,6 @@ lemma strong_right_of_misereOutcome_R {A : GameForm → Prop} [PFree A] [Outcome
       exact (misereOutcome_N_iff_miserePlayerOutcome.mp h6).right
     · exact winsGoingFirst_right_of_misereOutcome_R h6
   · exact winsGoingFirst_right_of_misereOutcome_R (OutcomeStable.misereOutcome_of_add_RR h1 hx h2 h5)
-
-private theorem reduction_ab_between_int_left.aux {a b : ℤ} (h0 : 0 ≤ a) (h1 : a + 2 ≤ b)
-    : !{{(a : GameForm)}|{(b : GameForm)}} ≥m PFreeDeadEnding !{{((b - 2 : ℤ) : GameForm)}|{1}} := by
-  apply Hereditary.misereGE_of_maintenance_proviso PFreeDeadEnding
-  · simp only [Maintenance, moves_ofSets, Set.mem_singleton_iff, exists_eq_left, forall_eq]
-    refine Or.inr ⟨(b - 1 : ℤ), leftMoves_intCast_zero_lt (by omega), ?_⟩
-    have h2 := reduction_ab_int (b - 2) 1 (by omega) Int.le_rfl (by omega)
-    rw [Form.intCast_ofNat, Nat.cast_one] at h2
-    apply misereGE_rw_right h2
-    have h3 : b - 2 + 1 = b - 1 := by omega
-    rw [h3]
-    exact MisereGE.refl _
-  · simp only [Maintenance, moves_ofSets, Set.mem_singleton_iff, exists_eq_left, forall_eq]
-    exact Or.inl (misereGE_of_int_le (b - 2) a (by omega))
-  · simp [Proviso, isEnd_def]
-  · simp [Proviso, isEnd_def]
-
-theorem reduction_ab_between_int_left {a b : ℤ} (h0 : 0 ≤ a) (h1 : a + 2 ≤ b)
-    : !{{(a : GameForm)}|{(b : GameForm)}} ≥m PFreeDeadEnding ((b - 1 : ℤ) : GameForm) := by
-  refine misereGE_rw_right (MisereEQ.symm ?_) (reduction_ab_between_int_left.aux h0 h1)
-  have h2 := reduction_ab_int (b - 2) 1 (by omega) Int.le_rfl (by omega)
-  have h4 : b - 2 + 1 = b - 1 := by omega
-  rwa [Form.intCast_ofNat, Nat.cast_one, h4] at h2
-
-theorem reduction_ab_between_int_right {a b : ℤ} (h0 : 0 ≤ a) (h1 : 1 ≤ b)
-    : ((a + 1 : ℤ) : GameForm) ≥m PFreeDeadEnding !{{(a : GameForm)}|{(b : GameForm)}} := by
-  refine misereGE_rw_left ?_ (reduction_ab_int.auxR a h1)
-  have h2 := reduction_ab_int a 1 h0 Int.le_rfl (by omega)
-  norm_cast at h2
-
-private theorem reduction_a_eq_neg_ba_c.aux {a b : ℤ} (h1 : 0 ≤ a) (h2 : 0 < b)
-    : !{{-(b : GameForm)} | {((a + 1 : ℤ) : GameForm)}} ≥m PFreeDeadEnding (a : GameForm) := by
-  apply misereGE_of_maintenance_proviso ?_ (HasInt.has_int _)
-  · simp [Maintenance]
-    apply Or.inr
-    use a
-    simp [leftMoves_intCast_zero_le_succ h1]
-  · simp only [Maintenance, moves_ofSets, Player.cases, Set.mem_singleton_iff, exists_eq_left]
-    intro x h5
-    apply Or.inl
-    obtain h_lt | h_eq := lt_or_eq_of_le h1
-    · simp only [leftMoves_intCast h_lt, Set.mem_singleton_iff] at h5
-      rw [h5, <-Form.intCast_neg]
-      exact misereGE_of_int_le _ _ (by omega)
-    · simp [h_eq] at h5
-  · simp [isEnd_def]
-  · intro h5 h6
-    have : a = 0 := by exact Eq.symm (Int.le_antisymm h1 (isEnd_left_intCast_iff.mp h5))
-    subst this
-    rw [misereOutcome_R_iff_winsGoingFirst] at h6
-    absurd h6.right
-    apply winsGoingFirst_of_moves
-    use -b
-    constructor
-    · simp only [zero_add, Form.intCast_ofNat, Nat.cast_one, leftMoves_ofSets, Set.mem_singleton_iff]
-    · rw [not_winsGoingFirst_iff]
-      simp [h2]
-      rw [<-Form.intCast_neg, winsGoingFirst_left_intCast_iff]
-      omega
-  · unfold IsPFree
-    constructor
-    · intro h3
-      rw [misereOutcome_P_iff_winsGoingFirst] at h3
-      absurd h3.right
-      apply winsGoingFirst_of_moves
-      simp [h2, <-Form.intCast_neg]
-    · intro p gp h_gp
-      cases p
-      <;> simp only [leftMoves_ofSets, rightMoves_ofSets, Set.mem_singleton_iff] at h_gp
-      <;> simp only [h_gp, isPFree_intCast, ClosedUnderNeg.neg_iff]
-
-theorem reduction_a_eq_neg_ba_c {a b c : ℤ} (h1 : 1 ≤ a) (h2 : 1 ≤ b) (h3 : 1 ≤ c) (h4 : c ≤ a + 1)
-    : !{{!{{(((-b) : ℤ) : GameForm)}|{(a : GameForm)}}}|{(c : GameForm)}} =m PFreeDeadEnding (a : GameForm)  := by
-  obtain ⟨a', h5⟩ := Int.le.dest h1
-  norm_cast at h5
-  rw [add_comm] at h5
-  rw [<-h5]; norm_cast
-  have h6 := reduction_ab_int a' 1 (Int.natCast_nonneg a') Int.le_rfl (by omega)
-  rw [Form.intCast_nat] at h6
-  refine MisereEQ.trans ?_ h6
-  refine MisereEq.of_antisymm ?_ ?_
-  · apply Hereditary.misereGE_of_maintenance_proviso PFreeDeadEnding
-    · simp only [Maintenance, moves_ofSets, Player.cases, Set.mem_singleton_iff,
-                 exists_eq_left, forall_eq]
-      apply Or.inr
-      use (c - 1 : ℤ), leftMoves_intCast_zero_lt h3
-      apply misereGE_rw_right h6
-      exact misereGE_of_int_le _ _ (by omega)
-    · simp only [Maintenance, Form.intCast_ofNat, Nat.cast_one, moves_ofSets,
-                 Player.cases, Set.mem_singleton_iff, Form.intCast_neg, Nat.cast_add, exists_eq_left,
-                 forall_eq, rightMoves_natCast, Set.mem_empty_iff_false, false_and,
-                 exists_const, or_false]
-      have h3 := reduction_a_eq_neg_ba_c.aux (Int.natCast_nonneg a') h2
-      norm_cast at h3
-      norm_cast
-    · simp [Proviso, isEnd_def]
-    · simp [Proviso, isEnd_def]
-  · apply Hereditary.misereGE_of_maintenance_proviso PFreeDeadEnding
-    · simp only [Maintenance, moves_ofSets, Player.cases, Set.mem_singleton_iff, Form.intCast_neg,
-                 exists_eq_left, forall_eq]
-      apply Or.inl
-      exact misereGE_of_int_le _ _ h3
-    · simp only [Maintenance, Form.intCast_neg, Nat.cast_one,
-                 moves_ofSets, Player.cases, Set.mem_singleton_iff, Form.intCast_ofNat, exists_eq_left,
-                 forall_eq]
-      apply Or.inr
-      norm_cast at h6
-      apply misereGE_rw_left (MisereEQ.symm h6)
-      exact MisereGE.refl ((a' + 1) : GameForm)
-    · simp [Proviso, isEnd_def]
-    · simp [Proviso, isEnd_def]
 
 private theorem misereEQ_intCast_pred_of_options {g : GameForm.{u}} (n : ℤ) (hn : n ≤ 0)
     (h_isEnd : IsEnd .left g)
@@ -483,7 +307,7 @@ private theorem isEnd_left_exists_intCast_misereEQ {g : GameForm}
     subst h_g_eq_zero
     intro x _
     simp
-  · have h_isDeadEnd_g := isDeadEnd_of_isDeadEnding h_g.isDeadEnding h_isEnd_left
+  · have h_isDeadEnd_g := isDeadEnd_of_isDeadEnding (DeadEnding.isDeadEnding h_g) h_isEnd_left
     have h_opt : ∀ gr ∈ moves .right g,
         ∃ n : ℕ, gr =m PFreeDeadEnding ((-(n : ℤ) : ℤ) : GameForm) := by
       intro gr h_gr
@@ -518,495 +342,3 @@ theorem isEnd_exists_intCast_misereEQ {p : Player} {g : GameForm} (h_g : PFreeDe
     exact ⟨-(a : ℤ), ha⟩
   · obtain ⟨a, ha⟩ := isEnd_right_exists_intCast_misereEQ h_g h_isEnd
     exact ⟨(a : ℤ), ha⟩
-
-/--
-Combination of `reduction_a_one_int` with `IntegerInvertible.zero_misereEQ_minusOne_one`.
--/
-theorem reduction_pred_one_int {n : ℤ} (h_n : 0 ≤ n) :
-    (!{{((n - 1 : ℤ) : GameForm)} | {1}}) =m PFreeDeadEnding ((n : ℤ) : GameForm) := by
-  rcases h_n.lt_or_eq with h1 | h0
-  · -- `1 ≤ n`
-    have h := reduction_a_one_int (a := n - 1) (by omega)
-    have he : (n - 1 + 1 : ℤ) = n := by omega
-    rwa [he] at h
-  · -- `n = 0`
-    subst h0
-    simp [IntegerInvertible.zero_misereEQ_minusOne_one.symm]
-
--- TODO: Move somewhere
-theorem pfreeSubset_short_ofSets {L R : Set GameForm} [Small.{u} L] [Small.{u} R]
-    {A : GameForm → Prop} [ClosedUnderDicotic IsShort A] [Short A]
-    (h_L_mem : ∀ gl ∈ L, (PFreeSubset A) gl) (h_R_mem : ∀ gr ∈ R, (PFreeSubset A) gr)
-    (h_L_nonempty : L.Nonempty) (h_L_finite : L.Finite)
-    (h_R_nonempty : R.Nonempty) (h_R_finite : R.Finite)
-    (h_outcome_ne_P : MisereOutcome (!{L | R}) ≠ .P) :
-    (PFreeSubset A) (!{L | R}) := by
-  have h_moves : ∀ p x, x ∈ moves p (!{L | R}) → (PFreeSubset A) x := by
-    intro p x h_x_mem
-    cases p
-    · rw [leftMoves_ofSets] at h_x_mem; exact h_L_mem x h_x_mem
-    · rw [rightMoves_ofSets] at h_x_mem; exact h_R_mem x h_x_mem
-  apply PFreeSubset.mk
-  · refine ClosedUnderDicotic.closed_dicotic (IsAmbient := IsShort)
-             L R ?_ ?_ h_L_nonempty h_R_nonempty ?_
-    · intro gl h_gl_mem
-      exact (h_L_mem gl h_gl_mem).mem
-    · intro gr h_gr_mem
-      exact (h_R_mem gr h_gr_mem).mem
-    · refine IsShort.ofSets h_L_finite ?_ h_R_finite ?_
-      · intro gl h_gl_mem
-        exact Short.isShort (h_L_mem gl h_gl_mem).mem
-      · intro gr h_gr_mem
-        exact Short.isShort (h_R_mem gr h_gr_mem).mem
-  · unfold IsPFree
-    refine ⟨h_outcome_ne_P, ?_⟩
-    intro p gp h_gp_mem
-    exact (h_moves p gp h_gp_mem).isPFree
-
--- TODO: This may generalize to blocking
-private theorem rightSeparating_of_leftSeparating {g h : GameForm}
-    (h_h : IsShort h) (h_left : AreLeftSeparating PFreeDeadEnding g h) :
-    AreRightSeparating PFreeDeadEnding g h := by
-  obtain ⟨x, h_x_pf, h_not_wins_left, h_wins_left⟩ := h_left
-  set L : Set GameForm :=
-    Set.range (fun r : moves .right h => (-((LTippingPoint (Hereditary.of_mem_moves h_h r.prop)))))
-    ∪ {((-1 : ℤ) : GameForm)} with h_L_def
-  have h_conj_one_mem : ((-1 : ℤ) : GameForm) ∈ L := Set.mem_union_right _ (Set.mem_singleton _)
-  have h_x_mem : x ∈ moves .right (!{L | {x}} : GameForm) := by simp
-  have := (misereOutcome_L_intCast_iff (G := GameForm) (-1)).mpr (by decide)
-  have h_not_wins_right : ¬ WinsGoingFirst .right (((-1 : ℤ) : GameForm)) :=
-    (misereOutcome_L_iff_winsGoingFirst.mp this).2
-  refine ⟨!{L | {x}}, ?_, ?_, ?_⟩
-  · apply pfreeSubset_short_ofSets
-    · intro a h_a_mem
-      rw [h_L_def] at h_a_mem
-      rcases h_a_mem with ⟨r, rfl⟩ | rfl
-      · exact HasInt.has_neg_int (A := PFreeDeadEnding) _
-      · exact HasInt.has_int (A := PFreeDeadEnding) (-1)
-    · intro a h_a_mem
-      rw [Set.mem_singleton_iff] at h_a_mem
-      subst h_a_mem
-      exact h_x_pf
-    · exact ⟨_, h_conj_one_mem⟩
-    · rw [h_L_def]
-      have := IsShort.finite_moves' .right h_h
-      simp [Set.finite_range]
-    · exact ⟨x, Set.mem_singleton x⟩
-    · exact Set.finite_singleton x
-    · intro h_outcome_P
-      rw [misereOutcome_P_iff_winsGoingFirst' (p := .left)] at h_outcome_P
-      refine h_outcome_P.left (winsGoingFirst_of_moves ⟨((-1 : ℤ) : GameForm), ?_, ?_⟩)
-      · rwa [leftMoves_ofSets]
-      · rwa [Player.neg_left]
-  · refine winsGoingFirst_of_moves ⟨g + x, add_left_mem_moves_add h_x_mem g, ?_⟩
-    rwa [Player.neg_right]
-  · rw [not_winsGoingFirst_iff]
-    refine ⟨?_, ?_⟩
-    · simp [isEnd_def]
-    · intro k h_k_mem
-      rw [moves_add] at h_k_mem
-      rw [Player.neg_right]
-      rcases h_k_mem with ⟨h_r, h_r_mem, rfl⟩ | ⟨r, h_r_mem, rfl⟩
-      · apply winsGoingFirst_of_moves
-        use h_r + (-(LTippingPoint (Hereditary.of_mem_moves h_h h_r_mem)))
-        constructor
-        · apply add_left_mem_moves_add
-          rw [leftMoves_ofSets, h_L_def]
-          exact Set.mem_union_left _ ⟨⟨h_r, h_r_mem⟩, rfl⟩
-        · rw [Player.neg_left]
-          have := LTippingPoint_spec (Hereditary.of_mem_moves h_h h_r_mem)
-          rw [misereOutcome_L_iff_winsGoingFirst] at this
-          exact this.right
-      · rw [rightMoves_ofSets, Set.mem_singleton_iff] at h_r_mem
-        subst h_r_mem
-        exact h_wins_left
-
-/--
-$(G, H)$ are Right $\operatorname{pf}(\mathcal{E})$-separated if and only if
-$(G, H)$ are Left $\operatorname{pf}(\mathcal{E})$-separated.
--/
-theorem rightSeparating_iff_leftSeparating {g h : GameForm} (h_g : IsShort g) (h_h : IsShort h) :
-    AreRightSeparating PFreeDeadEnding g h ↔ AreLeftSeparating PFreeDeadEnding g h := by
-  constructor
-  · intro h_right
-    have h1 := Separation.leftSeparating_neg_of_rightSeparating h_right
-    have h2 := rightSeparating_of_leftSeparating
-      (ClosedUnderNeg.neg_of h_g) h1
-    simpa using Separation.leftSeparating_neg_of_rightSeparating h2
-  · exact rightSeparating_of_leftSeparating h_h
-
-/--
-$\operatorname{pf}(\mathcal{E})$ is a separating set.
--/
-instance : Separating IsShort PFreeDeadEnding where
-  separating_pair_of_not_misereGE h_g h_h h_not_ge := by
-    rcases not_misereGE_iff_separating.mp h_not_ge with h_left | h_right
-    · rw [rightSeparating_iff_leftSeparating h_g h_h]
-      exact ⟨h_left, h_left⟩
-    · rw [<-rightSeparating_iff_leftSeparating h_g h_h]
-      exact ⟨h_right, h_right⟩
-
--- TODO: This could be generalized once we have [Short A]
-private theorem downlinked_intCast_of_not_leftMoves_misereGE {g : GameForm} {n : ℤ}
-    (h_g : PFreeDeadEnding g) (h_not_left_end : ¬ IsEnd .left g) (h_n : 0 ≤ n)
-    (h : ∀ gl ∈ moves .left g, ¬ (gl ≥m PFreeDeadEnding ((n : ℤ) : GameForm))) :
-    Form.Downlinked PFreeDeadEnding g ((n : ℤ) : GameForm) := by
-  have h_sep : ∀ gl, gl ∈ moves .left g → ∃ y : GameForm, PFreeDeadEnding y ∧
-      ¬ WinsGoingFirst .left (gl + y) ∧ WinsGoingFirst .left (((n : ℤ) : GameForm) + y) := by
-    intro gl h_gl_mem
-    exact (Separating.separating_pair_of_not_misereGE
-      (IsShort.of_mem_moves (Short.isShort h_g) h_gl_mem) (IsShort.intCast n) (h _ h_gl_mem)).1
-  choose x h_x_mem h_glx_win_left h_ngl_win_left using h_sep
-  set R : Set GameForm := Set.range (fun gl : (moves .left g) => x gl.1 gl.2) with hR_def
-  set t : GameForm := !{{((-1 : ℤ) : GameForm)} | R} with ht_def
-  have h_t_leftMoves : moves .left t = {((-1 : ℤ) : GameForm)} := by rw [ht_def, leftMoves_ofSets]
-  have h_t_rightMoves : moves .right t = R := by rw [ht_def, rightMoves_ofSets]
-  have h_t_mem : PFreeDeadEnding t := by
-    rw [ht_def]
-    refine pfreeSubset_short_ofSets ?_ ?_
-      (Set.singleton_nonempty _) (Set.finite_singleton _) ?_ ?_ ?_
-    · intro a ha; rw [Set.mem_singleton_iff] at ha; subst ha; exact HasInt.has_int (-1 : ℤ)
-    · rintro a ⟨⟨gl, hgl⟩, rfl⟩; exact h_x_mem gl hgl
-    · obtain ⟨gl, h_gl_mem⟩ := not_isEnd_exists_move h_not_left_end
-      exact ⟨x gl h_gl_mem, ⟨gl, h_gl_mem⟩, rfl⟩
-    · have : Finite (moves .left g) := IsShort.finite_moves' .left (Short.isShort h_g)
-      exact Set.toFinite _
-    · intro h_outcome_P
-      rw [misereOutcome_P_iff_winsGoingFirst] at h_outcome_P
-      absurd h_outcome_P.right
-      refine (winsGoingFirst_of_moves ⟨((-1 : ℤ) : GameForm), ?_, ?_⟩)
-      · rw [leftMoves_ofSets]; exact Set.mem_singleton _
-      · refine (misereOutcome_L_iff_winsGoingFirst.mp ?_).right
-        rw [misereOutcome_L_intCast_iff]
-        exact neg_one_lt_zero
-  use t, h_t_mem
-  constructor
-  · rw [not_winsGoingFirst_iff]
-    refine ⟨?_, ?_⟩
-    · rw [GameForm.isEndLike_iff_isEnd]
-      exact fun hend => h_not_left_end (IsEnd.add_iff.mp hend).1
-    · intro p hp
-      rw [moves_add] at hp
-      rcases hp with ⟨gl, hgl, rfl⟩ | ⟨tl, htl, rfl⟩
-      · refine winsGoingFirst_of_moves ⟨gl + x gl hgl, ?_, h_glx_win_left gl hgl⟩
-        refine add_left_mem_moves_add (?_ : x gl hgl ∈ moves Player.right t) gl
-        rw [h_t_rightMoves]
-        exact ⟨⟨gl, hgl⟩, rfl⟩
-      · rw [h_t_leftMoves, Set.mem_singleton_iff] at htl; subst htl
-        exact OutcomeStable.winsGoingFirst_right_sub_one_of_not_leftMoves_misereGE
-            h_g (Short.isShort h_g) h_not_left_end h_n h
-  · rw [not_winsGoingFirst_iff]
-    constructor
-    · rw [GameForm.isEndLike_iff_isEnd]
-      intro h_nt_isEnd
-      have h_t_isEnd : IsEnd .right t := (IsEnd.add_iff.mp h_nt_isEnd).right
-      rw [isEnd_def, h_t_rightMoves] at h_t_isEnd
-      simp only [hR_def, Set.range_eq_empty_iff, Set.isEmpty_coe_sort, ←isEnd_def] at h_t_isEnd
-      exact h_not_left_end h_t_isEnd
-    · intro ntr h_ntr_mem
-      rw [moves_add] at h_ntr_mem
-      rcases h_ntr_mem with ⟨nr, hnr, rfl⟩ | ⟨tr, htr, rfl⟩
-      · exfalso
-        have h_n_isEnd : IsEnd Player.right ((n : ℤ) : GameForm) := isEnd_right_intCast_iff.mpr h_n
-        rw [isEnd_def] at h_n_isEnd
-        rw [h_n_isEnd] at hnr
-        exact (Set.mem_empty_iff_false nr).mp hnr
-      · rw [h_t_rightMoves] at htr; obtain ⟨⟨gl, h_gl_mem⟩, rfl⟩ := htr
-        exact h_ngl_win_left gl h_gl_mem
-
-private lemma maintenance_of_misereGE_int_left
-    {g : GameForm} {n : ℤ} (h_n : 0 ≤ n)
-    (h_g : PFreeDeadEnding g) (g_not_end : ¬IsEnd .left g)
-    (h_ge : g ≥m PFreeDeadEnding (n : ℤ)) :
-    Maintenance PFreeDeadEnding g !{{((n - 1 : ℤ) : GameForm)} | {1}} .left := by
-  intro hl h_hl_mem
-  rw [leftMoves_ofSets, Set.mem_singleton_iff] at h_hl_mem
-  subst h_hl_mem
-  rcases h_n.lt_or_eq with h_zero_lt | h_zero_eq_n
-  · apply Or.inl
-    by_contra h_contra
-    push_neg at h_contra
-    have h_downlinked :=
-      downlinked_intCast_of_not_leftMoves_misereGE (n := n - 1) h_g g_not_end (by omega) h_contra
-    have h_mem : ((n - 1 : ℤ) : GameForm) ∈ moves .left ((n : ℤ) : GameForm) :=
-      leftMoves_intCast_zero_lt h_zero_lt
-    absurd h_downlinked
-    exact Form.not_downlinked_left_option_of_misereGE h_ge h_mem
-  · subst h_zero_eq_n
-    apply Or.inr
-    refine ⟨(0 : GameForm), ?_, ?_⟩
-    · simp
-    · simpa using h_ge
-
-private lemma maintenance_of_misereGE_int_right
-    {g : GameForm} {n : ℤ} (h_n : 0 ≤ n)
-    (h_g : PFreeDeadEnding g) (h_ge : g ≥m PFreeDeadEnding (n : ℤ)) :
-    Maintenance PFreeDeadEnding g !{{((n - 1 : ℤ) : GameForm)} | {1}} .right := by
-  intro gr h_gr_mem
-  by_contra h_contra
-  push_neg at h_contra
-  have : Downlinked PFreeDeadEnding gr ((n : ℤ) : GameForm) := by
-    refine downlinked_intCast_of_not_leftMoves_misereGE (n := n)
-      (Hereditary.of_mem_moves h_g h_gr_mem) ?_ h_n ?_
-    · intro hgr_left_end
-      have hgr_not_ge : ¬ gr ≥m PFreeDeadEnding ((1 : ℤ) : GameForm) := by
-        apply h_contra.left
-        simp only [rightMoves_ofSets, Form.intCast_ofNat, Nat.cast_one, Set.mem_singleton_iff]
-      obtain ⟨k, hk⟩ :=
-        isEnd_left_exists_intCast_misereEQ (Hereditary.of_mem_moves h_g h_gr_mem) hgr_left_end
-      have := PFreeDeadEnding.misereGE_of_int_le 1 (-(k : ℤ)) (by omega)
-      have := (misereGE_rw_left (MisereEQ.symm hk) this)
-      exact hgr_not_ge this
-    · intro grl hgrl h_gl_ge
-      have := (misereGE_rw_right (reduction_pred_one_int h_n) h_gl_ge)
-      exact h_contra.right grl hgrl this
-  absurd this
-  exact Form.not_downlinked_right_option_of_misereGE h_ge h_gr_mem
-
-/--
-If $G \in \operatorname{pf}(\mathcal{E})$ is not a Left end
-and $n \ge_{\mathbb{Z}} 0$, then
-$G \ge_{\operatorname{pf}(\mathcal{E})} n$ if and only if $(G, \{n - 1 \mid 1\})$ satisfy
-proviso and maintenance.
-
-Recall that $n =_{\operatorname{pf}(\mathcal{E})} \{n - 1 \mid 1\}$ by `reduction_pred_one_int`.
--/
-theorem misereGE_iff_promain_not_isEnd_left_int {g : GameForm} {n : ℤ} (h_n : 0 ≤ n)
-    (h_g : PFreeDeadEnding g) (h_g_not_isEnd : ¬IsEnd .left g) :
-    (g ≥m PFreeDeadEnding (n : ℤ) ↔
-      (Promain.Test PFreeDeadEnding g !{{((n - 1 : ℤ) : GameForm)} | {1}})) := by
-  constructor
-  · intro h_ge
-    unfold Promain.Test
-    have := misereGE_rw_right (reduction_pred_one_int h_n) h_ge
-    exact ⟨ maintenance_of_misereGE_int_right h_n h_g h_ge
-          , maintenance_of_misereGE_int_left h_n h_g h_g_not_isEnd h_ge
-          , proviso_right_of_misereGE this
-          , proviso_left_of_misereGE this
-          ⟩
-  · intro ⟨h1, h2, h3, h4⟩
-    have := MisereEQ.symm (reduction_pred_one_int h_n)
-    apply misereGE_rw_right this
-    refine Hereditary.misereGE_of_maintenance_proviso PFreeDeadEnding h1 h2 h3 h4
-
-private theorem downlinked_of_witness {g h t : GameForm}
-    (h_g_not_isEnd : ¬ IsEnd .left g) (h_h_not_isEnd : ¬ IsEnd .right h)
-    (h_t_mem : PFreeDeadEnding t)
-    (x : ∀ gl ∈ moves .left g, GameForm) (y : ∀ hr ∈ moves .right h, GameForm)
-    (h_x_g : ∀ gl (h : gl ∈ moves .left g), ¬ WinsGoingFirst .left (gl + x gl h))
-    (h_y_h : ∀ hr (h : hr ∈ moves .right h), ¬ WinsGoingFirst .right (hr + y hr h))
-    (h_x_mem : ∀ gl (h : gl ∈ moves .left g), x gl h ∈ moves .right t)
-    (h_y_mem : ∀ hr (h : hr ∈ moves .right h), y hr h ∈ moves .left t)
-    (h_t_left_win : ∀ tl ∈ moves .left t, WinsGoingFirst .right (g + tl))
-    (h_t_right_win : ∀ tr ∈ moves .right t, WinsGoingFirst .left (h + tr)) :
-    Form.Downlinked PFreeDeadEnding g h := by
-  use t, h_t_mem
-  constructor
-  · rw [not_winsGoingFirst_iff]
-    refine ⟨?_, ?_⟩
-    · rw [GameForm.isEndLike_iff_isEnd, IsEnd.add_iff]
-      intro h1
-      exact h_g_not_isEnd h1.left
-    · intro gtl h_gtl_mem
-      rw [moves_add] at h_gtl_mem
-      rw [Player.neg_left]
-      rcases h_gtl_mem with ⟨gl, h_gl_mem, rfl⟩ | ⟨tl, h_tl_mem, rfl⟩
-      · refine winsGoingFirst_of_moves ⟨gl + x gl h_gl_mem, ?_, ?_⟩
-        · exact add_left_mem_moves_add (h_x_mem gl h_gl_mem) gl
-        · rw [Player.neg_right]
-          exact h_x_g gl h_gl_mem
-      · exact h_t_left_win tl h_tl_mem
-  · rw [not_winsGoingFirst_iff]
-    refine ⟨?_, ?_⟩
-    · rw [GameForm.isEndLike_iff_isEnd, IsEnd.add_iff]
-      exact fun h => h_h_not_isEnd h.1
-    · intro htr h_htr_mem
-      rw [moves_add] at h_htr_mem
-      rw [Player.neg_right]
-      rcases h_htr_mem with ⟨hr, h_hr_mem, rfl⟩ | ⟨tr, h_tr_mem, rfl⟩
-      · refine winsGoingFirst_of_moves ⟨hr + y hr h_hr_mem, ?_, ?_⟩
-        · exact add_left_mem_moves_add (h_y_mem hr h_hr_mem) hr
-        · rw [Player.neg_left]
-          exact h_y_h hr h_hr_mem
-      · exact h_t_right_win tr h_tr_mem
-
-private theorem downlinked_of_misereOutcome_ne_L {g h : GameForm}
-    (h_g : PFreeDeadEnding g) (h_h : PFreeDeadEnding h)
-    (h_g_not_isEnd : ¬ IsEnd .left g) (h_h_not_isEnd : ¬ IsEnd .right h)
-    (h_moves_g : ∀ gl ∈ moves .left g, ¬ (gl ≥m PFreeDeadEnding h))
-    (h_moves_h : ∀ hr ∈ moves .right h, ¬ (g ≥m PFreeDeadEnding hr))
-    (h_outcome_ne_L : MisereOutcome (g + ((-1 : ℤ) : GameForm)) ≠ .L) :
-    Form.Downlinked PFreeDeadEnding g h := by
-  choose x h_x_mem h_x_g_win h_x_h_win using fun gl (h_gl_mem : gl ∈ moves .left g) =>
-    (Separating.separating_pair_of_not_misereGE
-      (IsShort.of_mem_moves (Short.isShort h_g) h_gl_mem) (Short.isShort h_h) (h_moves_g gl h_gl_mem)).left
-  choose y h_y_mem h_y_g_win h_y_h_win using fun hr (h_hr_mem : hr ∈ moves .right h) =>
-    (Separating.separating_pair_of_not_misereGE (Short.isShort h_g)
-      (IsShort.of_mem_moves (Short.isShort h_h) h_hr_mem) (h_moves_h hr h_hr_mem)).right
-  set L : Set GameForm := Set.range (fun hr : moves .right h => y hr.val hr.prop) with hLset_def
-  set R : Set GameForm := Set.range (fun gl : moves .left g => x gl.val gl.prop) with hRset_def
-  set t : GameForm := !{{((-1 : ℤ) : GameForm)} ∪ L | R} with hw_def
-  have h_t_leftMoves : moves .left t = {((-1 : ℤ) : GameForm)} ∪ L := by
-    rw [hw_def, leftMoves_ofSets]
-  have h_t_rightMoves : moves .right t = R := by
-    rw [hw_def, rightMoves_ofSets]
-  have h_t_pf : PFreeDeadEnding t := by
-    apply pfreeSubset_short_ofSets
-    · rintro gl (rfl | ⟨hr, rfl⟩)
-      · exact HasInt.has_int (-1 : ℤ)
-      · exact h_y_mem _ _
-    · rintro gr ⟨gl, rfl⟩
-      exact h_x_mem _ _
-    · exact ⟨_, Set.mem_union_left _ (Set.mem_singleton _)⟩
-    · have : Finite (moves .right h) := IsShort.finite_moves' .right (Short.isShort h_h)
-      exact (Set.finite_singleton _).union (Set.finite_range _)
-    · obtain ⟨gl, h_gl_mem⟩ := not_isEnd_exists_move h_g_not_isEnd
-      exact ⟨_, ⟨⟨gl, h_gl_mem⟩, rfl⟩⟩
-    · have : Finite (moves .left g) := IsShort.finite_moves' .left (Short.isShort h_g)
-      exact Set.finite_range _
-    · intro h_outcome_P
-      rw [misereOutcome_P_iff_winsGoingFirst] at h_outcome_P
-      absurd h_outcome_P.right
-      refine winsGoingFirst_of_moves ⟨((-1 : ℤ) : GameForm), ?_, ?_⟩
-      · rw [h_t_leftMoves]; exact Set.mem_union_left _ (Set.mem_singleton _)
-      · rw [<-winsGoingFirst_neg_iff]
-        simp
-  apply downlinked_of_witness h_g_not_isEnd h_h_not_isEnd h_t_pf x y h_x_g_win h_y_h_win
-  · intro gl h_gl_mem; rw [h_t_rightMoves]; exact ⟨⟨gl, h_gl_mem⟩, rfl⟩
-  · intro hr h_hr_mem; rw [h_t_leftMoves]; exact Set.mem_union_right _ ⟨⟨hr, h_hr_mem⟩, rfl⟩
-  · intro tl h_tl_mem
-    rw [h_t_leftMoves] at h_tl_mem
-    rcases h_tl_mem with (rfl | ⟨tr, rfl⟩)
-    · cases ho : MisereOutcome (g + ((-1 : ℤ) : GameForm)) with
-      | L => exact absurd ho h_outcome_ne_L
-      | P => exact absurd ho (OutcomeStable.misereOutcome_add_int_ne_P h_g (-1))
-      | N => exact (misereOutcome_N_iff_winsGoingFirst.mp ho).right
-      | R => exact (misereOutcome_R_iff_winsGoingFirst.mp ho).left
-    · exact h_y_g_win _ _
-  · intro tr h_tr_mem
-    rw [h_t_rightMoves] at h_tr_mem
-    obtain ⟨⟨gl, h_gl_mem⟩, rfl⟩ := h_tr_mem
-    exact h_x_h_win gl h_gl_mem
-
-private theorem downlinked_of_misereOutcome_eq_L {g h : GameForm}
-    (h_g : PFreeDeadEnding g) (h_h : PFreeDeadEnding h)
-    (h_g_not_isEnd : ¬ IsEnd .left g) (h_h_not_isEnd : ¬ IsEnd .right h)
-    (h_moves_g : ∀ gl ∈ moves .left g, ¬ (gl ≥m PFreeDeadEnding h))
-    (h_moves_h : ∀ hr ∈ moves .right h, ¬ (g ≥m PFreeDeadEnding hr))
-    (h_outcome_eq_L : MisereOutcome (g + ((-1 : ℤ) : GameForm)) = .L) :
-    Form.Downlinked PFreeDeadEnding g h := by
-  choose x h_x_mem h_x_g_win h_x_h_win using fun gl (h_gl_mem : gl ∈ moves .left g) =>
-    (Separating.separating_pair_of_not_misereGE
-      (IsShort.of_mem_moves (Short.isShort h_g) h_gl_mem) (Short.isShort h_h) (h_moves_g gl h_gl_mem)).left
-  choose y h_y_mem h_y_g_win h_y_h_win using fun hr (h_hr_mem : hr ∈ moves .right h) =>
-    (Separating.separating_pair_of_not_misereGE (Short.isShort h_g)
-      (IsShort.of_mem_moves (Short.isShort h_h) h_hr_mem) (h_moves_h hr h_hr_mem)).right
-  set L : Set GameForm := Set.range (fun hr : moves .right h => y hr.val hr.prop) with hLset_def
-  set R : Set GameForm := Set.range (fun gl : moves .left g => x gl.val gl.prop) with hRset_def
-  set t : GameForm := !{L | R} with hw_def
-  have h_t_leftMoves : moves .left t = L := by
-    rw [hw_def, leftMoves_ofSets]
-  have h_t_rightMoves : moves .right t = R := by
-    rw [hw_def, rightMoves_ofSets]
-  have h_t_pf : PFreeDeadEnding t := by
-    apply pfreeSubset_short_ofSets
-    · rintro gl ⟨hr, rfl⟩
-      exact h_y_mem _ _
-    · rintro gr ⟨gl, rfl⟩
-      exact h_x_mem _ _
-    · obtain ⟨hr, h_hr_mem⟩ := not_isEnd_exists_move h_h_not_isEnd
-      exact ⟨_, ⟨⟨hr, h_hr_mem⟩, rfl⟩⟩
-    · have : Finite (moves .right h) := IsShort.finite_moves' .right (Short.isShort h_h)
-      exact Set.finite_range _
-    · obtain ⟨gl, h_gl_mem⟩ := not_isEnd_exists_move h_g_not_isEnd
-      exact ⟨_, ⟨⟨gl, h_gl_mem⟩, rfl⟩⟩
-    · have : Finite (moves .left g) := IsShort.finite_moves' .left (Short.isShort h_g)
-      exact Set.finite_range _
-    · intro h_outcome_P
-      rw [misereOutcome_P_iff_winsGoingFirst] at h_outcome_P
-      absurd h_outcome_P.left
-      obtain ⟨gl, h_gl_mem, h_gl_ge_zero⟩ :=
-        OutcomeStable.exists_leftMove_misereGE_zero_of_misereOutcome_add_neg_one_L
-          h_g h_g_not_isEnd h_outcome_eq_L
-      refine winsGoingFirst_of_moves ⟨x gl h_gl_mem, ?_, ?_⟩
-      · rw [h_t_rightMoves]; exact ⟨⟨gl, h_gl_mem⟩, rfl⟩
-      · rw [Player.neg_right]
-        intro h
-        have := winsGoingFirst_left_add_of_misereGE_zero (h_x_mem gl h_gl_mem) h_gl_ge_zero h
-        apply h_x_g_win gl h_gl_mem this
-  apply downlinked_of_witness h_g_not_isEnd h_h_not_isEnd h_t_pf x y h_x_g_win h_y_h_win
-  · intro gl h_gl_mem; rw [h_t_rightMoves]; exact ⟨⟨gl, h_gl_mem⟩, rfl⟩
-  · intro hr h_hr_mem; rw [h_t_leftMoves]; exact ⟨⟨hr, h_hr_mem⟩, rfl⟩
-  · intro tl h_tl_mem
-    rw [h_t_leftMoves] at h_tl_mem
-    obtain ⟨⟨tr, h_tr_mem⟩, rfl⟩ := h_tl_mem
-    exact h_y_g_win tr h_tr_mem
-  · intro wr hwr
-    rw [h_t_rightMoves] at hwr
-    obtain ⟨⟨gl, h_gl_mem⟩, rfl⟩ := hwr
-    exact h_x_h_win gl h_gl_mem
-
-theorem downlinked_of_not_isEnd_left
-    {g h : GameForm} (h_g : PFreeDeadEnding g) (h_h : PFreeDeadEnding h)
-    (h_g_not_isEnd : ¬ IsEnd .left g)
-    (h_moves_g : ∀ gl ∈ moves .left g, ¬ (gl ≥m PFreeDeadEnding h))
-    (h_moves_h : ∀ hr ∈ moves .right h, ¬ (g ≥m PFreeDeadEnding hr)) :
-    Downlinked PFreeDeadEnding g h := by
-  by_cases h_t_right : IsEnd .right h
-  · obtain ⟨n, hn⟩ := isEnd_right_exists_intCast_misereEQ h_h h_t_right
-    have h_gl : ∀ gl ∈ gᴸ, ¬ (gl ≥m PFreeDeadEnding ((n : ℤ) : GameForm)) :=
-      fun sl hsl h => h_moves_g sl hsl (misereGE_rw_right hn h)
-    apply downlinked_of_downlinked_misereEQ_right hn.symm
-    exact downlinked_intCast_of_not_leftMoves_misereGE h_g h_g_not_isEnd (Int.natCast_nonneg n) h_gl
-  · by_cases hL : MisereOutcome (g + ((-1 : ℤ) : GameForm)) = .L
-    · exact downlinked_of_misereOutcome_eq_L h_g h_h h_g_not_isEnd h_t_right h_moves_g h_moves_h hL
-    · exact downlinked_of_misereOutcome_ne_L h_g h_h h_g_not_isEnd h_t_right h_moves_g h_moves_h hL
-
-theorem downlinked_of_not_isEnd_right
-    {g h : GameForm} (h_g : PFreeDeadEnding g) (h_h : PFreeDeadEnding h)
-    (h_h_not_isEnd : ¬ IsEnd .right h)
-    (h_moves_g : ∀ gl ∈ moves .left g, ¬ (gl ≥m PFreeDeadEnding h))
-    (h_moves_h : ∀ hr ∈ moves .right h, ¬ (g ≥m PFreeDeadEnding hr)) :
-    Downlinked PFreeDeadEnding g h := by
-  rw [←Downlinked.neg_iff]
-  apply downlinked_of_not_isEnd_left (ClosedUnderNeg.neg_of h_h) (ClosedUnderNeg.neg_of h_g)
-  · rw [IsEnd.neg_iff_neg]
-    simpa using h_h_not_isEnd
-  · intro hl h_hl_neg_mem h_hl_ge
-    rw [moves_neg, Set.mem_neg] at h_hl_neg_mem
-    have := h_moves_h (-hl) h_hl_neg_mem
-    exact this ((ClosedUnderNeg.neg_ge_neg_iff g (-hl)).mp (by rwa [neg_neg]))
-  · intro gr h_gr_neg_mem h_gr_ge
-    rw [moves_neg, Set.mem_neg] at h_gr_neg_mem
-    have := h_moves_g (-gr) h_gr_neg_mem
-    exact this ((ClosedUnderNeg.neg_ge_neg_iff (-gr) h).mp (by rwa [neg_neg]))
-
-/--
-If $G \in \operatorname{pf}(\mathcal{E})$ is not a Left end
-and $H \in \operatorname{pf}(\mathcal{E})$ is not a Right end, then
-$G \ge_{\operatorname{pf}(\mathcal{E})} H$ if and only if $(G, H)$ satisfy proviso and maintenance.
--/
-theorem misereGE_iff_promain_not_isEnd_left_right
-    {g h : GameForm}
-    (h_g : PFreeDeadEnding g) (h_h : PFreeDeadEnding h)
-    (h_g_not_isEnd : ¬ IsEnd .left g) (h_h_not_isEnd : ¬ IsEnd .right h) :
-    g ≥m PFreeDeadEnding h ↔ Promain.Test PFreeDeadEnding g h := by
-  constructor
-  · intro hge
-    refine ⟨?_, ?_, proviso_right_of_misereGE hge, proviso_left_of_misereGE hge⟩
-    · intro gr h_gr_mem
-      by_contra h_not
-      push_neg at h_not
-      obtain ⟨h_no_hr, h_no_grl⟩ := h_not
-      have h_dl := downlinked_of_not_isEnd_right (Hereditary.of_mem_moves h_g h_gr_mem)
-        h_h h_h_not_isEnd h_no_grl h_no_hr
-      exact not_downlinked_right_option_of_misereGE hge h_gr_mem h_dl
-    · intro hl h_hl_mem
-      by_contra h_not
-      push_neg at h_not
-      obtain ⟨h_no_gl, h_no_hlr⟩ := h_not
-      have h_dl := downlinked_of_not_isEnd_left h_g (Hereditary.of_mem_moves h_h h_hl_mem)
-        h_g_not_isEnd h_no_gl h_no_hlr
-      exact not_downlinked_left_option_of_misereGE hge h_hl_mem h_dl
-  · intro ⟨h1, h2, h3, h4⟩
-    exact Hereditary.misereGE_of_maintenance_proviso PFreeDeadEnding h1 h2 h3 h4
